@prefix rdf: <http://www.w3.org/1999/02/22-rdf-syntax-ns#> .
@prefix rdfs: <http://www.w3.org/2000/01/rdf-schema#> .
@prefix qb: <http://purl.org/linked-data/cube#> .
@prefix owl: <http://www.w3.org/2002/07/owl#> .
@prefix hobbit: <http://w3id.org/hobbit/vocab#> .
@prefix exp: <http://w3id.org/hobbit/experiments#> .
@prefix xsd: <http://www.w3.org/2001/XMLSchema#> .
@prefix bench: <http://w3id.org/bench#> .
# --- Benchmark ---
bench:Linking a	hobbit:Benchmark;
	rdfs:label "Linking Benchmark"@en;
	rdfs:comment	"WP4.1 HOBBIT Linking Benchmark"@en;
# 	hobbit:imageName	"git.project-hobbit.eu:4567/jsaveta1/linkingbenchmarkcontroller";
 	hobbit:imageName	"linking_benchmark-controller";
	hobbit:hasAPI	bench:LinkingAPI ;
	hobbit:version "V1.1";
	hobbit:measuresKPI bench:precision ;
	hobbit:measuresKPI bench:recall ;
	hobbit:measuresKPI bench:fmeasure ;
	hobbit:measuresKPI bench:timePerformance ;
	hobbit:hasParameter	bench:hasPopulation;
	hobbit:hasParameter	bench:hasNumberOfGenerators;
        hobbit:hasParameter bench:linkingDataFormat ;
        hobbit:hasParameter bench:keepPoints ;        
        hobbit:hasParameter bench:severity ;
        hobbit:hasParameter bench:addRemovePoints ;
        hobbit:hasParameter bench:targetPointsTransformations;
        hobbit:hasParameter bench:valueBasedTransformations;
        hobbit:hasParameter bench:changeTimestamp ;
        hobbit:hasParameter bench:sourcePointsToLabels .

		
bench:LinkingAPI a hobbit:API .
# --- metrics ---
bench:precision a hobbit:KPI;
rdfs:label "Precision"@en;
	rdfs:comment	"Precision = TP / (TP + FP)"@en;
	rdfs:range	xsd:float .
bench:recall a hobbit:KPI;
rdfs:label "Recall"@en;
	rdfs:comment	"Recall = TP / (TP + FN)"@en;
	rdfs:range	xsd:float .
bench:fmeasure a hobbit:KPI;
rdfs:label "F-measure"@en;
	rdfs:comment	"F-measure is the harmonic mean of precision and recall."@en;
	rdfs:range	xsd:float .
	
bench:timePerformance a hobbit:KPI;
rdfs:label "timePerformance"@en;
	rdfs:comment	"Measures time needed for the system to return the results"@en;
	rdfs:range	xsd:float .
	
# --- parameters ---	
bench:hasPopulation	a	hobbit:Parameter, hobbit:FeatureParameter, hobbit:ConfigurableParameter;
        rdfs:label	"Population of generated data (number on instances)"@en;
        rdfs:comment	"Number of different events to be generated by a mimicking algorithm"@en;
        rdfs:domain	hobbit:Experiment, hobbit:Challenge;
        rdfs:range	xsd:unsignedInt;
        hobbit:defaultValue	"10"^^xsd:unsignedInt .
        
bench:hasNumberOfGenerators	a	hobbit:Parameter, hobbit:FeatureParameter, hobbit:ConfigurableParameter;
        rdfs:label	"Number of generators"@en;
        rdfs:domain	hobbit:Experiment, hobbit:Challenge;
        rdfs:range	xsd:unsignedInt;
        hobbit:defaultValue	"1"^^xsd:unsignedInt .
        
bench:keepPoints	a	hobbit:Parameter, hobbit:FeatureParameter, hobbit:ConfigurableParameter;
        rdfs:label	"Percentage of points to keep"@en;
        rdfs:comment	"The percentage should be smaller or equal to 1.0"@en;
        rdfs:domain	hobbit:Experiment, hobbit:Challenge;
        rdfs:range	xsd:float;
        hobbit:defaultValue	"1.0"^^xsd:float .
        
bench:sourcePointsToLabels	a	hobbit:Parameter, hobbit:FeatureParameter, hobbit:ConfigurableParameter;
        rdfs:label	"Points to labels"@en;
        rdfs:comment	"Percentage of points to be transformed to labels"@en;
        rdfs:domain	hobbit:Experiment, hobbit:Challenge;
        rdfs:range	xsd:float;
        hobbit:defaultValue	"0.4"^^xsd:float .
        
bench:severity	a	hobbit:Parameter, hobbit:FeatureParameter, hobbit:ConfigurableParameter;
        rdfs:label	"Difficulty of the transformations"@en;
        rdfs:comment	"The percentage should be smaller or equal to 1.0"@en;
        rdfs:domain	hobbit:Experiment, hobbit:Challenge;
        rdfs:range	xsd:float;
        hobbit:defaultValue	"0.3"^^xsd:float .
        
bench:changeTimestamp	a	hobbit:Parameter, hobbit:FeatureParameter, hobbit:ConfigurableParameter;
        rdfs:label	"Timestamp format "@en;
        rdfs:comment	"Percentage of timestamps to change format "@en;
        rdfs:domain	hobbit:Experiment, hobbit:Challenge;
        rdfs:range	xsd:float;
        hobbit:defaultValue	"0.1"^^xsd:float .
        
bench:addRemovePoints	a	hobbit:Parameter, hobbit:FeatureParameter, hobbit:ConfigurableParameter;
        rdfs:label	"Addition/Deletion of points. The sum of percentages should be smaller or equal to 1.0 and NOTRANSFORMATION should not be 0.0. Percentages define: ADDPOINTS, REMOVEPOINTS, NOTRANSFORMATION"@en;
        rdfs:comment	"Defines the allocation of adding and deleting points (traces). Do not give a high percentage on remove points, this can delete whole instances. The sum of percentages should be smaller or equal to 1.0 and NOTRANSFORMATION should not be 0.0"@en;
        rdfs:domain	hobbit:Experiment, hobbit:Challenge;
        rdfs:range	xsd:string;
        hobbit:defaultValue	"0.1, 0.1, 0.8" .
        
bench:targetPointsTransformations	a	hobbit:Parameter, hobbit:FeatureParameter, hobbit:ConfigurableParameter;
        rdfs:label	"Transform point to labels or change point format (for the target dataset). The sum of percentages should be smaller or equal to 1.0 and NOTRANSFORMATION should not be 0.0. Percentages define: CHANGECOORDINATES, POINTSTOLABEL,  NOTRANSFORMATION"@en;
        rdfs:comment	"Defines the allocation of transforming point to labels or changing point format (for the target dataset). The sum of percentages should be smaller or equal to 1.0 and NOTRANSFORMATION should not be 0.0"@en;
        rdfs:domain	hobbit:Experiment, hobbit:Challenge;
        rdfs:range	xsd:string;
        hobbit:defaultValue	"0.0, 0.3, 0.7" .

        
bench:valueBasedTransformations	a	hobbit:Parameter, hobbit:FeatureParameter, hobbit:ConfigurableParameter;
        rdfs:label	"Apply value-based transformations of labels of the source dataset. The sum of percentages should be smaller or equal to 1.0 and NOTRANSFORMATION should not be 0.0. Percentages define:  BLANKCHARSADDITION , BLANKCHARSDELETION ,RANDOMCHARSADDITION , RANDOMCHARSDELETION , RANDOMCHARSMODIFIER, TOKENADDITION, TOKENDELETION, TOKENSHUFFLE, NAMESTYLEABBREVIATION,  NOTRANSFORMATION"@en;
        rdfs:comment	"Defines the allocation of value based transformations. The sum of percentages should be smaller or equal to 1.0 and NOTRANSFORMATION should not be 0.0"@en;
        rdfs:domain	hobbit:Experiment, hobbit:Challenge;
        rdfs:range	xsd:string;
        hobbit:defaultValue	"0.05, 0.05, 0.1, 0.1, 0.1, 0.1, 0.1, 0.1, 0.1, 0.2" .
        
# --- output data format ---
bench:linkingDataFormat  a	hobbit:Parameter, hobbit:FeatureParameter, hobbit:ConfigurableParameter;
				rdfs:label		"Generated data format"@en;
				rdfs:comment		"The serialization format in which the generated data will be saved."@en;
				rdfs:domain		hobbit:Experiment, hobbit:Challenge;
				rdfs:range		bench:DataFormat;
				hobbit:defaultValue	bench:Turtle .
				
bench:DataFormat    a   rdfs:Class, owl:Class .
bench:NTriples           a   bench:DataFormat;
                    rdfs:label "NTriples"@en;
                    rdfs:comment "Data will be generated in N-Triples Serialization format"@en .
bench:NQuads           a   bench:DataFormat;
                    rdfs:label "NQuads"@en;
                    rdfs:comment "Data will be generated in N-Quads Serialization format"@en .
bench:N3           a   bench:DataFormat;
                    rdfs:label "N3"@en;
                    rdfs:comment "Data will be egenerated in N3 Serialization format"@en .
bench:RDFXML           a   bench:DataFormat;
                    rdfs:label "RDFXML"@en;
                    rdfs:comment "Data will be generated in RDF/XML Serialization format"@en .
bench:Turtle           a   bench:DataFormat;
                    rdfs:label "Turtle"@en;
                    rdfs:comment "Data will be generated in Turtle Serialization format"@en .
bench:Trig           a   bench:DataFormat;
                    rdfs:label "TriG"@en;
                    rdfs:comment "Data will be generated in TriG Serialization format"@en .
bench:TriX           a   bench:DataFormat;
                    rdfs:label "TriX"@en;
                    rdfs:comment "Data will begenerated in TriX Serialization format"@en .
bench:RDFJSON           a   bench:DataFormat;
                    rdfs:label "RDFJSON"@en;
                    rdfs:comment "Data generated in RDF/JSON Serialization format"@en .
